AP/Util/Data/Raw/RawData.lean
@@ -12,15 +12,15 @@ inductive Valid : RawData → Prop where
 | lit : {n : ℕ} → Valid (lit n)
 | mp : {xs : List _} → xs.Sorted (·.1 < ·.1) → (∀ x ∈ xs, x.2.Valid) → Valid (mp xs)
 
-#check 0 #exit
+-- #check 0 #exit
 
-def depth (d : RawData) : ℕ :=
-  @d.recOn (λ _ => ℕ) (λ _ => List ℕ) (λ _ => ℕ)
-  (λ _ => 0) (λ _ xs => 1 + xs.max?.getD 0) []
-  (λ _ _ n ns => n :: ns) (λ _ _ n => n)
+-- def depth (d : RawData) : ℕ :=
+--   @d.recOn (λ _ => ℕ) (λ _ => List ℕ) (λ _ => ℕ)
+--   (λ _ => 0) (λ _ xs => 1 + xs.max?.getD 0) []
+--   (λ _ _ n ns => n :: ns) (λ _ _ n => n)
 
-#check 0 #exit
+-- #check 0 #exit
 
-def valid : RawData → Bool
-| lit _ => true
-| mp xs => xs.Sorted (·.1 < ·.1) && xs.all (·.2.valid)
+-- def valid : RawData → Bool
+-- | lit _ => true
+-- | mp xs => xs.Sorted (·.1 < ·.1) && xs.all (·.2.valid)
