AP/Sokoban/Card.lean
@@ -1,0 +1,16 @@
+import AP.Sokoban.Basic
+
+namespace Sokoban
+
+private structure FinSTate (w h : ℕ) where
+  mp : Map (Fin w × Fin h) Tile
+
+-- private def State.supReach (s : State) : Finset State := List.toFinset do
+--   let grid ← do
+--   { s with
+--     grid := grid
+--   }
+-- 
+-- theorem finite_reachable {s : State} [hs : s.Valid] :
+-- {s' | sys.Reachable s s'}.Finite := by
+--   apply Set.finite_of_subset_finset (s := s.supReach)
