AP/Sokoban/Main.lean
@@ -1,1 +1,1 @@
-import AP.Sokoban.Basic
+import AP.Sokoban.Card
