AP/Util/Data/Raw/RawChange.lean
@@ -1,4 +1,4 @@
 import AP.Util.Data.Raw.RawData
 
-inductive RawChange where
-| exact : RawData → RawChange
+-- inductive RawChange where
+-- | exact : RawData → RawChange
