AP/Util/Multiset.lean
@@ -2,8 +2,8 @@ import Mathlib.Data.Finset.Union
 import Mathlib.Data.Multiset.Fold
 import Mathlib.Data.Multiset.Count
 
-import AP.Util.Quotient
 import AP.Util.List
+import AP.Util.Quotient
 
 namespace Multiset
 
